ulib/LowStar.Monotonic.Buffer.fsti
@@ -25,7 +25,7 @@ unfold let srel (a:Type0) = Seq.seq_pre a
 /// type ``u``, then Low* type ``buffer t`` is translated to C type ``u*``.
 ///
 /// The type is indexed by two preorders:
-/// rrel is the starting preorder with which the original buffer was initially created
+/// rrel is the preorder with which the original buffer was initially created
 /// rel  is the preorder of the current buffer (which could be a sub-buffer of the original one)
 ///
 /// The buffer contents are constrained to evolve according to rel
@@ -46,9 +46,9 @@ val mbuffer (a:Type0) (rrel rel:srel a) :Tot Type0
 
 val g_is_null (#a:Type0) (#rrel #rel:srel a) (b:mbuffer a rrel rel) :GTot bool
 
-val null (#a:Type0) (#rrel #rel:srel a) :Tot (b:mbuffer a rrel rel {g_is_null b})
+val mnull (#a:Type0) (#rrel #rel:srel a) :Tot (b:mbuffer a rrel rel {g_is_null b})
 
-val null_unique (#a:Type0) (#rrel #rel:srel a) (b:mbuffer a rrel rel) :Lemma (g_is_null b <==> b == null)
+val null_unique (#a:Type0) (#rrel #rel:srel a) (b:mbuffer a rrel rel) :Lemma (g_is_null b <==> b == mnull)
 
 /// ``unused_in b h`` holds only if buffer ``b`` has not been allocated
 /// yet.
@@ -76,7 +76,7 @@ val live (#a:Type0) (#rrel #rel:srel a) (h:HS.mem) (b:mbuffer a rrel rel) :GTot 
 
 /// The null pointer is always live.
 
-val live_null (a:Type0) (rrel rel:srel a) (h:HS.mem) :Lemma (live h (null #a #rrel #rel))
+val live_null (a:Type0) (rrel rel:srel a) (h:HS.mem) :Lemma (live h (mnull #a #rrel #rel))
 
 let live_is_null (#a:Type0) (#rrel #rel:srel a) (h:HS.mem) (b:mbuffer a rrel rel)
   :Lemma (requires (g_is_null b == true))
@@ -162,7 +162,7 @@ let length (#a:Type0) (#rrel #rel:srel a) (b:mbuffer a rrel rel) :GTot nat = U32
 
 /// The null pointer has length 0.
 
-val len_null (a:Type0) (rrel rel:srel a) :Lemma (len (null #a #rrel #rel) == 0ul)
+val len_null (a:Type0) (rrel rel:srel a) :Lemma (len (mnull #a #rrel #rel) == 0ul)
 
 let length_null_1 (#a:Type0) (#rrel #rel:srel a) (b:mbuffer a rrel rel)
   :Lemma (requires (length b =!= 0)) (ensures (g_is_null b == false))
@@ -225,11 +225,11 @@ let compatible_sub
 /// ``gsub`` is the ghost version, for proof purposes. Its stateful
 /// counterpart is ``sub``, see below.
 
-val gsub (#a:Type0) (#rrel #rel:srel a)
+val mgsub (#a:Type0) (#rrel #rel:srel a)
   (b:mbuffer a rrel rel) (i:U32.t) (len:U32.t) (sub_rel:srel a)
-  : Ghost (mbuffer a rrel sub_rel)
-          (requires (U32.v i + U32.v len <= length b /\ compatible_sub b i len sub_rel))
-	  (ensures (fun _ -> True))
+  :Ghost (mbuffer a rrel sub_rel)
+         (requires (U32.v i + U32.v len <= length b /\ compatible_sub b i len sub_rel))
+	 (ensures (fun _ -> True))
 
 // goffset
 
@@ -238,18 +238,18 @@ val gsub (#a:Type0) (#rrel #rel:srel a)
 val live_gsub (#a:Type0) (#rrel #rel:srel a)
   (h:HS.mem) (b:mbuffer a rrel rel) (i:U32.t) (len:U32.t) (sub_rel:srel a)
   :Lemma (requires (U32.v i + U32.v len <= length b /\ compatible_sub b i len sub_rel))
-         (ensures  (live h (gsub b i len sub_rel) <==> live h b))
+         (ensures  (live h (mgsub b i len sub_rel) <==> live h b))
          [SMTPatOr [
-             [SMTPat (live h (gsub b i len sub_rel))];
-             [SMTPat (live h b); SMTPat (gsub b i len sub_rel);]
+             [SMTPat (live h (mgsub b i len sub_rel))];
+             [SMTPat (live h b); SMTPat (mgsub b i len sub_rel);]
          ]]
 
 
 val gsub_is_null (#a:Type0) (#rrel #rel:srel a)
   (b:mbuffer a rrel rel) (i:U32.t) (len:U32.t) (sub_rel:srel a)
   :Lemma (requires (U32.v i + U32.v len <= length b /\ compatible_sub b i len sub_rel))
-         (ensures (g_is_null (gsub b i len sub_rel) <==> g_is_null b))
-         [SMTPat (g_is_null (gsub b i len sub_rel))]
+         (ensures (g_is_null (mgsub b i len sub_rel) <==> g_is_null b))
+         [SMTPat (g_is_null (mgsub b i len sub_rel))]
 
 
 /// The length of a sub-buffer is exactly the one provided at ``gsub``.
@@ -258,33 +258,33 @@ val gsub_is_null (#a:Type0) (#rrel #rel:srel a)
 val len_gsub (#a:Type0) (#rrel #rel:srel a)
   (b:mbuffer a rrel rel) (i:U32.t) (len':U32.t) (sub_rel:srel a)
   :Lemma (requires (U32.v i + U32.v len' <= length b /\ compatible_sub b i len' sub_rel))
-         (ensures (len (gsub b i len' sub_rel) == len'))
+         (ensures (len (mgsub b i len' sub_rel) == len'))
          [SMTPatOr [
-             [SMTPat (len (gsub b i len' sub_rel))];
-             [SMTPat (length (gsub b i len' sub_rel))];
+             [SMTPat (len (mgsub b i len' sub_rel))];
+             [SMTPat (length (mgsub b i len' sub_rel))];
          ]]
 
 
 val frameOf_gsub (#a:Type0) (#rrel #rel:srel a)
   (b:mbuffer a rrel rel) (i:U32.t) (len:U32.t) (sub_rel:srel a)
   :Lemma (requires (U32.v i + U32.v len <= length b /\ compatible_sub b i len sub_rel))
-         (ensures (frameOf (gsub b i len sub_rel) == frameOf b))
-  [SMTPat (frameOf (gsub b i len sub_rel))]
+         (ensures (frameOf (mgsub b i len sub_rel) == frameOf b))
+  [SMTPat (frameOf (mgsub b i len sub_rel))]
 
 val as_addr_gsub (#a:Type0) (#rrel #rel:srel a)
   (b:mbuffer a rrel rel) (i:U32.t) (len:U32.t) (sub_rel:srel a)
   :Lemma (requires (U32.v i + U32.v len <= length b /\ compatible_sub b i len sub_rel))
-         (ensures (as_addr (gsub b i len sub_rel) == as_addr b))
-         [SMTPat (as_addr (gsub b i len sub_rel))]
+         (ensures (as_addr (mgsub b i len sub_rel) == as_addr b))
+         [SMTPat (as_addr (mgsub b i len sub_rel))]
 
-val gsub_inj (#a:Type0) (#rrel #rel:srel a)
+val mgsub_inj (#a:Type0) (#rrel #rel:srel a)
   (b1 b2:mbuffer a rrel rel)
   (i1 i2:U32.t)
   (len1 len2:U32.t)
   (sub_rel1 sub_rel2:srel a)
   :Lemma (requires (U32.v i1 + U32.v len1 <= length b1 /\ compatible_sub b1 i1 len1 sub_rel1 /\
                     U32.v i2 + U32.v len2 <= length b2 /\ compatible_sub b2 i2 len2 sub_rel2 /\
-		    gsub b1 i1 len1 sub_rel1 === gsub b2 i2 len2 sub_rel2))
+		    mgsub b1 i1 len1 sub_rel1 === mgsub b2 i2 len2 sub_rel2))
          (ensures (len1 == len2 /\ (b1 == b2 ==> i1 == i2) /\ ((i1 == i2 /\ length b1 == length b2) ==> b1 == b2)))
 
 
@@ -295,17 +295,17 @@ val gsub_gsub (#a:Type0) (#rrel #rel:srel a)
   (i1:U32.t) (len1:U32.t) (sub_rel1:srel a)
   (i2: U32.t) (len2: U32.t) (sub_rel2:srel a)
   :Lemma (requires (U32.v i1 + U32.v len1 <= length b /\ compatible_sub b i1 len1 sub_rel1 /\
-                    U32.v i2 + U32.v len2 <= U32.v len1 /\ compatible_sub (gsub b i1 len1 sub_rel1) i2 len2 sub_rel2))
+                    U32.v i2 + U32.v len2 <= U32.v len1 /\ compatible_sub (mgsub b i1 len1 sub_rel1) i2 len2 sub_rel2))
          (ensures  (compatible_sub b (U32.add i1 i2) len2 sub_rel2 /\
-                    gsub (gsub b i1 len1 sub_rel1) i2 len2 sub_rel2 == gsub b (U32.add i1 i2) len2 sub_rel2))
-         [SMTPat (gsub (gsub b i1 len1 sub_rel1) i2 len2 sub_rel2)]
+                    mgsub (mgsub b i1 len1 sub_rel1) i2 len2 sub_rel2 == mgsub b (U32.add i1 i2) len2 sub_rel2))
+         [SMTPat (mgsub (mgsub b i1 len1 sub_rel1) i2 len2 sub_rel2)]
 
 
 /// A buffer ``b`` is equal to its "largest" sub-buffer, at index 0 and
 /// length ``len b``.
 
 val gsub_zero_length (#a:Type0) (#rrel #rel:srel a) (b:mbuffer a rrel rel)
-  :Lemma (compatible_sub b 0ul (len b) rel /\ b == gsub b 0ul (len b) rel)
+  :Lemma (compatible_sub b 0ul (len b) rel /\ b == mgsub b 0ul (len b) rel)
 
 
 /// The contents of a sub-buffer is the corresponding slice of the
@@ -314,8 +314,8 @@ val gsub_zero_length (#a:Type0) (#rrel #rel:srel a) (b:mbuffer a rrel rel)
 val as_seq_gsub (#a:Type0) (#rrel #rel:srel a)
   (h:HS.mem) (b:mbuffer a rrel rel) (i:U32.t) (len:U32.t) (sub_rel:srel a)
   :Lemma (requires (U32.v i + U32.v len <= length b /\ compatible_sub b i len sub_rel))
-         (ensures (as_seq h (gsub b i len sub_rel) == Seq.slice (as_seq h b) (U32.v i) (U32.v i + U32.v len)))
-         [SMTPat (as_seq h (gsub b i len sub_rel))]
+         (ensures (as_seq h (mgsub b i len sub_rel) == Seq.slice (as_seq h b) (U32.v i) (U32.v i + U32.v len)))
+         [SMTPat (as_seq h (mgsub b i len sub_rel))]
 
 /// # The modifies clause
 ///
@@ -395,8 +395,8 @@ val loc_union_loc_none_r
 val loc_buffer (#a:Type0) (#rrel #rel:srel a) (b:mbuffer a rrel rel) :GTot loc
 
 val loc_buffer_null (a:Type0) (rrel rel:srel a)
-  :Lemma (loc_buffer (null #a #rrel #rel) == loc_none)
-         [SMTPat (loc_buffer (null #a #rrel #rel))]
+  :Lemma (loc_buffer (mnull #a #rrel #rel) == loc_none)
+         [SMTPat (loc_buffer (mnull #a #rrel #rel))]
 
 /// ``loc_addresses r n`` is the set of memory locations associated to a
 /// set of addresses ``n`` in a given region ``r``.
@@ -537,14 +537,14 @@ val loc_includes_gsub_buffer_r
 : Lemma (requires (UInt32.v i + UInt32.v len <= (length b) /\
                    compatible_sub b i len sub_rel /\
                    loc_includes l (loc_buffer b)))
-        (ensures  (loc_includes l (loc_buffer (gsub b i len sub_rel))))
-        [SMTPat (loc_includes l (loc_buffer (gsub b i len sub_rel)))]
+        (ensures  (loc_includes l (loc_buffer (mgsub b i len sub_rel))))
+        [SMTPat (loc_includes l (loc_buffer (mgsub b i len sub_rel)))]
 
 let loc_includes_gsub_buffer_r' (#a:Type0) (#rrel #rel:srel a)
   (b:mbuffer a rrel rel) (i:UInt32.t) (len:UInt32.t) (sub_rel:srel a)
   :Lemma (requires (UInt32.v i + UInt32.v len <= (length b) /\ compatible_sub b i len sub_rel))
-         (ensures  (loc_includes (loc_buffer b) (loc_buffer (gsub b i len sub_rel))))
-         [SMTPat (gsub b i len sub_rel)]
+         (ensures  (loc_includes (loc_buffer b) (loc_buffer (mgsub b i len sub_rel))))
+         [SMTPat (mgsub b i len sub_rel)]
   = ()
 
 val loc_includes_gsub_buffer_l (#a:Type0) (#rrel #rel:srel a) (b:mbuffer a rrel rel)
@@ -553,8 +553,8 @@ val loc_includes_gsub_buffer_l (#a:Type0) (#rrel #rel:srel a) (b:mbuffer a rrel 
   :Lemma (requires (UInt32.v i1 + UInt32.v len1 <= (length b) /\
                     UInt32.v i1 <= UInt32.v i2 /\ UInt32.v i2 + UInt32.v len2 <= UInt32.v i1 + UInt32.v len1 /\
 		    compatible_sub b i1 len1 sub_rel1 /\ compatible_sub b i2 len2 sub_rel2))
-         (ensures  (loc_includes (loc_buffer (gsub b i1 len1 sub_rel1)) (loc_buffer (gsub b i2 len2 sub_rel2))))
-         [SMTPat (gsub b i1 len1 sub_rel1); SMTPat (gsub b i2 len2 sub_rel2)]
+         (ensures  (loc_includes (loc_buffer (mgsub b i1 len1 sub_rel1)) (loc_buffer (mgsub b i2 len2 sub_rel2))))
+         [SMTPat (mgsub b i1 len1 sub_rel1); SMTPat (mgsub b i2 len2 sub_rel2)]
 
 /// If the contents of a buffer are equal in two given heaps, then so
 /// are the contents of any of its sub-buffers.
@@ -818,8 +818,8 @@ val loc_disjoint_gsub_buffer (#a:Type0) (#rrel:srel a) (#rel:srel a)
 		    compatible_sub b i1 len1 sub_rel1 /\ compatible_sub b i2 len2 sub_rel2 /\
 		    (UInt32.v i1 + UInt32.v len1 <= UInt32.v i2 \/
                      UInt32.v i2 + UInt32.v len2 <= UInt32.v i1)))
-         (ensures  (loc_disjoint (loc_buffer (gsub b i1 len1 sub_rel1)) (loc_buffer (gsub b i2 len2 sub_rel2))))
-         [SMTPat (gsub b i1 len1 sub_rel1); SMTPat (gsub b i2 len2 sub_rel2)]
+         (ensures  (loc_disjoint (loc_buffer (mgsub b i1 len1 sub_rel1)) (loc_buffer (mgsub b i2 len2 sub_rel2))))
+         [SMTPat (mgsub b i1 len1 sub_rel1); SMTPat (mgsub b i2 len2 sub_rel2)]
 
 
 /// If two sets of addresses correspond to different regions or are
@@ -1613,11 +1613,11 @@ val is_null (#a:Type0) (#rrel #rel:srel a) (b:mbuffer a rrel rel)
 /// offset ``i`` with length ``len``. KreMLin extracts this operation as
 /// ``b + i`` (or, equivalently, ``&b[i]``.)
 
-val sub (#a:Type0) (#rrel #rel:srel a) (b:mbuffer a rrel rel)
+val msub (#a:Type0) (#rrel #rel:srel a) (b:mbuffer a rrel rel)
   (i:U32.t) (len:U32.t) (sub_rel:srel a)
   :HST.Stack (mbuffer a rrel sub_rel)
              (requires (fun h -> U32.v i + U32.v len <= length b /\ compatible_sub b i len sub_rel /\ live h b))
-             (ensures  (fun h y h' -> h == h' /\ y == gsub b i len sub_rel))
+             (ensures  (fun h y h' -> h == h' /\ y == mgsub b i len sub_rel))
 
 
 /// ``offset b i`` construct the tail of the buffer ``b`` starting from
@@ -1628,11 +1628,11 @@ val sub (#a:Type0) (#rrel #rel:srel a) (b:mbuffer a rrel rel)
 /// This stateful operation cannot be derived from ``sub``, because the
 /// length cannot be computed outside of proofs.
 
-val offset (#a:Type0) (#rrel #rel:srel a) (b:mbuffer a rrel rel)
+val moffset (#a:Type0) (#rrel #rel:srel a) (b:mbuffer a rrel rel)
   (i:U32.t) (sub_rel:srel a)
   :HST.Stack (mbuffer a rrel sub_rel)
              (requires (fun h -> U32.v i <= length b /\ compatible_sub b i (U32.sub (len b) i) sub_rel /\ live h b))
-             (ensures  (fun h y h' -> h == h' /\ y == gsub b i (U32.sub (len b) i) sub_rel))
+             (ensures  (fun h y h' -> h == h' /\ y == mgsub b i (U32.sub (len b) i) sub_rel))
 // goffset
 
 
@@ -1713,7 +1713,7 @@ let upd
 val recallable (#a:Type0) (#rrel #rel:srel a) (b:mbuffer a rrel rel) :GTot Type0
 
 val recallable_null (#a:Type0) (#rrel #rel:srel a)
-  :Lemma (recallable (null #a #rrel #rel)) [SMTPat (recallable (null #a #rrel #rel))]
+  :Lemma (recallable (mnull #a #rrel #rel)) [SMTPat (recallable (mnull #a #rrel #rel))]
 
 val recallable_includes (#a1 #a2:Type0) (#rrel1 #rel1:srel a1) (#rrel2 #rel2:srel a2)
   (larger:mbuffer a1 rrel1 rel1) (smaller:mbuffer a2 rrel2 rel2)
@@ -1785,7 +1785,7 @@ let alloc_post_common (#a:Type0) (#rrel #rel:srel a)
 /// buffer will have initial contents ``init``. Such a buffer cannot be
 /// freed. In fact, it is eternal: it cannot be deallocated at all.
 
-val gcmalloc (#a:Type0) (#rrel:srel a)
+val mgcmalloc (#a:Type0) (#rrel:srel a)
   (r:HS.rid) (init:a) (len:U32.t)
   :HST.ST (b:mbuffer a rrel rrel{recallable b /\ alloc_post_static r (U32.v len) b})
           (requires (fun h -> HST.is_eternal_region r /\ U32.v len > 0))
@@ -1800,7 +1800,7 @@ val gcmalloc (#a:Type0) (#rrel:srel a)
 /// only on the whole buffer ``b``, and is not inherited by any of its
 /// strict sub-buffers.
 
-val malloc (#a:Type0) (#rrel:srel a)
+val mmalloc (#a:Type0) (#rrel:srel a)
   (r:HS.rid) (init:a) (len:U32.t)
   :HST.ST (mbuffer a rrel rrel)
           (requires (fun h -> HST.is_eternal_region r /\ U32.v len > 0))
@@ -1815,7 +1815,7 @@ val malloc (#a:Type0) (#rrel:srel a)
 /// individually, but is automatically freed as soon as its stack
 /// frame is deallocated by ``HST.pop_frame``.
 
-val alloca (#a:Type0) (#rrel:srel a)
+val malloca (#a:Type0) (#rrel:srel a)
   (init:a) (len:U32.t)
   :HST.StackInline (mbuffer a rrel rrel)
                    (requires (fun h -> U32.v len > 0))
@@ -1835,7 +1835,7 @@ unfold let alloc_of_list_pre (#a:Type0) (init:list a) :GTot Type0 =
 unfold let alloc_of_list_post (#a:Type0) (#rrel #rel:srel a) (len:nat) (buf:mbuffer a rrel rel) :GTot Type0 =
   normalize (length buf == len)
 
-val alloca_of_list (#a:Type0) (#rrel:srel a) (init: list a)
+val malloca_of_list (#a:Type0) (#rrel:srel a) (init: list a)
   :HST.StackInline (mbuffer a rrel rrel) (requires (fun h -> alloc_of_list_pre #a init))
                                          (ensures (fun h b h' -> let len = FStar.List.Tot.length init in
                                                                alloc_post_common (HS.get_tip h) len b h h' /\
@@ -1846,7 +1846,7 @@ unfold let gcmalloc_of_list_pre (#a:Type0) (init:list a) :GTot Type0 =
   normalize (FStar.List.Tot.length init <= UInt.max_int 32)
 
 (* TODO: Why is some of the post on the refinement? *)
-val gcmalloc_of_list (#a:Type0) (#rrel:srel a) (r:HS.rid) (init:list a)
+val mgcmalloc_of_list (#a:Type0) (#rrel:srel a) (r:HS.rid) (init:list a)
   :HST.ST (b:mbuffer a rrel rrel {
     let len = FStar.List.Tot.length init in
     recallable b /\
